demo/DemoBproof.v
@@ -1,5 +1,6 @@
 Require Import Coqlib Errors.
-Require Import AST Linking Smallstep.
+Require Import AST Linking Smallstep Invariant CallconvAlgebra.
+Require Import Conventions Mach.
 
 Require Import LanguageInterface.
 Require Import Asm Asmrel.
@@ -7,8 +8,109 @@ Require Import Asm Asmrel.
 Require Import Integers.
 Require Import SymbolTable DemoB DemoBspec.
 
-Require Import Compiler.
+Require Import CallConv Compiler.
+
+Require Import CKLRAlgebra Inject InjectFootprint.
+
+(** * Step1 : self_simulation of Bspec *)
+
+Section SELF_INJP.
+
+Theorem self_simulation_C :
+  forward_simulation (cc_c injp) (cc_c injp) Bspec Bspec.
+Proof.
+  constructor. econstructor; eauto. instantiate (1 := fun _ _ _ => _). cbn beta.
+  intros se1 se2 w Hse Hse1. cbn in *.
+  
+Admitted.
+
+End SELF_INJP.
+
+Section WT_C.
+
+Theorem self_simulation_wt :
+  forward_simulation (wt_c @ lessdef_c) (wt_c @ lessdef_c) Bspec Bspec.
+Proof.
+  constructor. econstructor; eauto. instantiate (1 := fun _ _ _ => _). cbn beta.
+  intros se1 se2 w Hse Hse1. cbn in *.
+  destruct w as [[se1' [se2' sg]] ?]. destruct Hse as [Hse Hse2].
+  subst. inv Hse.
+  eapply forward_simulation_step with (match_states:= eq).
+  - intros. inv H. inv H0. cbn in *.
+    inv H1. inv H. reflexivity.
+  - intros. inv H. inv H1. cbn in *. inv H. inv H1. exists s1.
+    split. inv H2. inv H0. simpl. simpl in *.
+    inv H. inv H2. inv H5.
+    econstructor; eauto. reflexivity.
+  - intros. subst.
+    inv H0. eexists.
+    split.
+    constructor.
+    eexists. split.
+    econstructor. simpl. admit. (*add WT assumptions in Bspec ?? How did they do for wt_c*)
+    econstructor. constructor.
+  - intros. subst.
+    exists (se2 , (se2, int_int_sg), tt).
+    exists q1. repeat apply conj; simpl; auto.
+    + exists q1. split; inv H0; simpl;  constructor; simpl; eauto.
+    + constructor; eauto. simpl. constructor. eauto.
+    + intros. exists s1'. split; eauto.
+      destruct H as [r3 [A B]].
+      inv A. inv B. inv H1. inv H2. constructor. auto.
+  - intros. subst. exists s1'. eauto.
+  - constructor. intros.
+    constructor. inv H.
+Admitted.
+
+End WT_C.
+
+Variable BspecL : Smallstep.semantics li_locset li_locset.
+Variable BspecM : Smallstep.semantics li_mach li_mach.
+Variable BspecA : Smallstep.semantics li_asm li_asm.
+
+Section CL.
+
+Theorem c_locset :
+  forward_simulation (cc_c_locset) (cc_c_locset) Bspec BspecL.
+Admitted.
+End CL.
+
+Section LM.
+
+Theorem locset_mach :
+  forward_simulation (cc_locset_mach) (cc_locset_mach) BspecL BspecM.
+Admitted.
+End LM.
+
+Section MA.
+
+Theorem mach_asm :
+  forward_simulation (cc_mach_asm) (cc_mach_asm) BspecM BspecA.
+Admitted.
+End MA.
+
+
+Section Ainj.
+
+Theorem asm_simulation_inj:
+  forward_simulation (cc_asm inj) (cc_asm inj) BspecA (Asm.semantics DemoB.prog).
+Admitted.
+
+End Ainj.
 
 Theorem Bproof :
   forward_simulation cc_compcert cc_compcert Bspec (Asm.semantics DemoB.prog).
-Admitted.
+Proof.
+  
+  unfold cc_compcert.
+  rewrite <- (cc_compose_assoc wt_c lessdef_c) at 1.
+  rewrite <- (cc_compose_assoc wt_c lessdef_c).
+  eapply compose_forward_simulations.
+  eapply self_simulation_C.
+  eapply compose_forward_simulations.
+  eapply self_simulation_wt.
+  repeat eapply compose_forward_simulations.
+  eapply c_locset. eapply locset_mach. eapply mach_asm.
+  eapply asm_simulation_inj.
+Qed.
+
